Switch to Iterator for Backtracker proof

correctness/RegexCorrectness/Backtracker/Traversal.lean
@@ -1,10 +1,12 @@
 import Regex.Strategy
+import RegexCorrectness.Data.BoundedIterator
 import RegexCorrectness.Backtracker.Basic
 import RegexCorrectness.Backtracker.Path
 
 set_option autoImplicit false
 
-open Regex.Data (Span BoundedIterator)
+open Regex.Data (BoundedIterator)
+open String (Iterator)
 
 namespace Regex.Backtracker.captureNextAux
 
@@ -127,7 +129,7 @@ Current candidates are:
 
 1. Closure under transition: ∀ (state, pos) ∈ visited, nfa.Step 0 state pos state' pos' → (state', pos') ∈ visited ∨ ∃ entry ∈ stack, entry.state = state' ∧ entry.it.poss = pos'
   * At the end of the traversal, we can use this invariant to show that the visited set is a reflexive-transitive closure of the step relation.
-2. Upper bound of the visited set: ∀ (state, pos) ∈ visited, (state, pos) ∈ visisted₀ ∨ ∃ span, Path nfa wf l r span state update
+2. Upper bound of the visited set: ∀ (state, pos) ∈ visited, (state, pos) ∈ visisted₀ ∨ ∃ it, Path nfa wf it₀ it state update
   * We'll strengthen `UpperInv` to give an upper bound of the visited set.
   * Combined with the closure property, we can show that the traversal adds just the states reachable from the starting node at a particular position.
 3. The visited set doesn't contain the `.done` state.
@@ -137,160 +139,152 @@ section
 
 variable {nfa wf startIdx maxIdx visited stack update' visited'}
 
-structure UpperInv (wf : nfa.WellFormed) (l r : List Char) (stack : List (StackEntry HistoryStrategy nfa startIdx maxIdx)) where
-  reachable : ∀ entry ∈ stack, ∃ span, span.iterator = entry.it.it ∧ Path nfa wf l r span entry.state entry.update
+structure UpperInv (wf : nfa.WellFormed) (it₀ : Iterator) (stack : List (StackEntry HistoryStrategy nfa startIdx maxIdx)) where
+  reachable : ∀ entry ∈ stack, Path nfa wf it₀ entry.it.it entry.state entry.update
 
-theorem path_done_of_some {l r} (hres : captureNextAux HistoryStrategy nfa wf startIdx maxIdx visited stack = (.some update', visited'))
-  (inv : UpperInv wf l r stack) :
-  ∃ state span, nfa[state] = .done ∧ Path nfa wf l r span state update' := by
+theorem path_done_of_some {it₀} (hres : captureNextAux HistoryStrategy nfa wf startIdx maxIdx visited stack = (.some update', visited'))
+  (inv : UpperInv wf it₀ stack) :
+  ∃ state it', nfa[state] = .done ∧ Path nfa wf it₀ it' state update' := by
   induction visited, stack using captureNextAux.induct' HistoryStrategy nfa wf startIdx with
   | base visited => simp [captureNextAux_base] at hres
   | visited visited update state it eq stack' mem ih =>
     simp [captureNextAux_visited mem] at hres
-    have inv' : UpperInv wf l r stack' := by
-      have reachable entry (mem : entry ∈ stack') : ∃ span, span.iterator = entry.it.it ∧ Path nfa wf l r span entry.state entry.update :=
+    have inv' : UpperInv wf it₀ stack' := by
+      have reachable entry (mem : entry ∈ stack') : Path nfa wf it₀ entry.it.it entry.state entry.update :=
         inv.reachable entry (by simp [mem])
       exact ⟨reachable⟩
     exact ih hres inv'
   | done visited update state it eq stack' mem hn =>
     simp [captureNextAux_done mem hn] at hres
-    have ⟨span, eqspan, path⟩ := inv.reachable ⟨update, state, it, eq⟩ (by simp)
-    exact ⟨state, span, hn, hres.1 ▸ path⟩
+    have path := inv.reachable ⟨update, state, it, eq⟩ (by simp)
+    exact ⟨state, it.it, hn, hres.1 ▸ path⟩
   | fail visited update state it eq stack' mem hn => simp [captureNextAux_fail mem hn] at hres
   | epsilon visited update state it eq stack' mem visited' state' hn ih =>
     rw [captureNextAux_epsilon mem hn] at hres
-    have inv' : UpperInv wf l r (⟨update, state', it, eq⟩ :: stack') := by
-      have reachable entry (mem : entry ∈ ⟨update, state', it, eq⟩ :: stack') : ∃ span, span.iterator = entry.it.it ∧ Path nfa wf l r span entry.state entry.update := by
+    have inv' : UpperInv wf it₀ (⟨update, state', it, eq⟩ :: stack') := by
+      have reachable entry (mem : entry ∈ ⟨update, state', it, eq⟩ :: stack') : Path nfa wf it₀ entry.it.it entry.state entry.update := by
         simp at mem
         cases mem with
         | inl eq' =>
-          subst entry
-          have ⟨span, eqspan, path⟩ := inv.reachable ⟨update, state, it, eq⟩ (by simp)
-          simp at eqspan path
-          exact ⟨span, by simp [eqspan], path.more (.epsilon (Nat.zero_le _) state.isLt hn) (by simp)⟩
+          simp [eq']
+          have path := inv.reachable ⟨update, state, it, eq⟩ (by simp)
+          simp at path
+          exact path.more (.epsilon (Nat.zero_le _) state.isLt hn path.validR) (by simp)
         | inr mem => exact inv.reachable entry (by simp [mem])
       exact ⟨reachable⟩
     exact ih hres inv'
   | split visited update state it eq stack' mem visited' state₁ state₂ hn ih =>
     rw [captureNextAux_split mem hn] at hres
     let stack'' := ⟨update, state₁, it, eq⟩ :: ⟨update, state₂, it, eq⟩ :: stack'
-    have inv' : UpperInv wf l r stack'' := by
-      have reachable entry (mem : entry ∈ stack'') : ∃ span, span.iterator = entry.it.it ∧ Path nfa wf l r span entry.state entry.update := by
+    have inv' : UpperInv wf it₀ stack'' := by
+      have reachable entry (mem : entry ∈ stack'') : Path nfa wf it₀ entry.it.it entry.state entry.update := by
         simp [stack''] at mem
         match mem with
         | .inl eq₁ =>
-          subst entry
-          have ⟨span, eqspan, path⟩ := inv.reachable ⟨update, state, it, eq⟩ (by simp)
-          simp at eqspan path
-          exact ⟨span, by simp [eqspan], path.more (.splitLeft (Nat.zero_le _) state.isLt hn) (by simp)⟩
+          simp [eq₁]
+          have path := inv.reachable ⟨update, state, it, eq⟩ (by simp)
+          simp at path
+          exact path.more (.splitLeft (Nat.zero_le _) state.isLt hn path.validR) (by simp)
         | .inr (.inl eq₂) =>
-          subst entry
-          have ⟨span, eqspan, path⟩ := inv.reachable ⟨update, state, it, eq⟩ (by simp)
-          simp at eqspan path
-          exact ⟨span, by simp [eqspan], path.more (.splitRight (Nat.zero_le _) state.isLt hn) (by simp)⟩
+          simp [eq₂]
+          have path := inv.reachable ⟨update, state, it, eq⟩ (by simp)
+          simp at path
+          exact path.more (.splitRight (Nat.zero_le _) state.isLt hn path.validR) (by simp)
         | .inr (.inr mem) => exact inv.reachable entry (by simp [mem])
       exact ⟨reachable⟩
     exact ih hres inv'
   | save visited update state it eq stack' mem visited' offset state' hn update' ih =>
     rw [captureNextAux_save mem hn] at hres
-    have inv' : UpperInv wf l r (⟨update', state', it, eq⟩ :: stack') := by
-      have reachable entry (mem : entry ∈ ⟨update', state', it, eq⟩ :: stack') : ∃ span, span.iterator = entry.it.it ∧ Path nfa wf l r span entry.state entry.update := by
+    have inv' : UpperInv wf it₀ (⟨update', state', it, eq⟩ :: stack') := by
+      have reachable entry (mem : entry ∈ ⟨update', state', it, eq⟩ :: stack') : Path nfa wf it₀ entry.it.it entry.state entry.update := by
         simp at mem
         cases mem with
         | inl eq' =>
-          subst entry
-          have ⟨span, eqspan, path⟩ := inv.reachable ⟨update, state, it, eq⟩ (by simp)
-          simp at eqspan path
-          exact ⟨span, by simp [eqspan], path.more (.save (Nat.zero_le _) state.isLt hn) (by simp [update', HistoryStrategy, BoundedIterator.pos, ←eqspan, Span.curr_eq_pos])⟩
+          simp [eq']
+          have path := inv.reachable ⟨update, state, it, eq⟩ (by simp)
+          simp at path
+          exact path.more (.save (Nat.zero_le _) state.isLt hn path.validR) (by simp [update', HistoryStrategy, BoundedIterator.pos])
         | inr mem => exact inv.reachable entry (by simp [mem])
       exact ⟨reachable⟩
     exact ih hres inv'
   | anchor_pos visited update state it eq stack' mem visited' a state' hn ht ih =>
     rw [captureNextAux_anchor_pos mem hn ht] at hres
-    have inv' : UpperInv wf l r (⟨update, state', it, eq⟩ :: stack') := by
-      have reachable entry (mem : entry ∈ ⟨update, state', it, eq⟩ :: stack') : ∃ span, span.iterator = entry.it.it ∧ Path nfa wf l r span entry.state entry.update := by
+    have inv' : UpperInv wf it₀ (⟨update, state', it, eq⟩ :: stack') := by
+      have reachable entry (mem : entry ∈ ⟨update, state', it, eq⟩ :: stack') : Path nfa wf it₀ entry.it.it entry.state entry.update := by
         simp at mem
         cases mem with
         | inl eq' =>
-          subst entry
-          have ⟨span, eqspan, path⟩ := inv.reachable ⟨update, state, it, eq⟩ (by simp)
-          simp at eqspan path
-          exact ⟨span, by simp [eqspan], path.more (.anchor (Nat.zero_le _) state.isLt hn (eqspan ▸ ht)) (by simp)⟩
+          simp [eq']
+          have path := inv.reachable ⟨update, state, it, eq⟩ (by simp)
+          simp at path
+          exact path.more (.anchor (Nat.zero_le _) state.isLt hn path.validR ht) (by simp)
         | inr mem => exact inv.reachable entry (by simp [mem])
       exact ⟨reachable⟩
     exact ih hres inv'
   | anchor_neg visited update state it eq stack' mem visited' a state' hn ht ih =>
     rw [captureNextAux_anchor_neg mem hn ht] at hres
-    have inv' : UpperInv wf l r stack' := by
-      have reachable entry (mem : entry ∈ stack') : ∃ span, span.iterator = entry.it.it ∧ Path nfa wf l r span entry.state entry.update :=
+    have inv' : UpperInv wf it₀ stack' := by
+      have reachable entry (mem : entry ∈ stack') : Path nfa wf it₀ entry.it.it entry.state entry.update :=
         inv.reachable entry (by simp [mem])
       exact ⟨reachable⟩
     exact ih hres inv'
   | char_pos visited update state it eq stack' mem visited' c state' hn hnext hc ih =>
     rw [captureNextAux_char_pos mem hn hnext hc] at hres
-    have inv' : UpperInv wf l r (⟨update, state', it.next hnext, eq⟩ :: stack') := by
-      have reachable entry (mem : entry ∈ ⟨update, state', it.next hnext, eq⟩ :: stack') : ∃ span, span.iterator = entry.it.it ∧ Path nfa wf l r span entry.state entry.update := by
+    have inv' : UpperInv wf it₀ (⟨update, state', it.next hnext, eq⟩ :: stack') := by
+      have reachable entry (mem : entry ∈ ⟨update, state', it.next hnext, eq⟩ :: stack') : Path nfa wf it₀ entry.it.it entry.state entry.update := by
         simp at mem
         cases mem with
         | inl eq' =>
-          subst entry
-          have ⟨span, eqspan, path⟩ := inv.reachable ⟨update, state, it, eq⟩ (by simp)
-          simp at eqspan path
-          simp [BoundedIterator.hasNext, BoundedIterator.curr, ←eqspan] at hnext hc
-          have ⟨r', eqr'⟩ := span.exists_cons_of_curr' hnext hc
-          refine ⟨span.next, by simp [span.next_iterator eqr', eqspan, BoundedIterator.next, String.Iterator.next'_eq_next], ?_⟩
-          simp
-          have step : NFA.Step nfa 0 state span state' span.next .none := by
-            simp [NFA.Step.iff_char hn, eqr', span.next_eq eqr']
-          exact path.more step (by simp)
+          simp [eq']
+          have path := inv.reachable ⟨update, state, it, eq⟩ (by simp)
+          simp at path
+          have v : it.Valid := it.valid_of_it_valid path.validR
+          have ⟨l, r, vf⟩ := v.validFor_of_hasNext hnext
+          exact path.more (.char (Nat.zero_le _) state.isLt hn (hc ▸ vf)) (by simp)
         | inr mem => exact inv.reachable entry (by simp [mem])
       exact ⟨reachable⟩
     exact ih hres inv'
   | char_neg visited update state it eq stack' mem visited' c state' hn hnext hc ih =>
     rw [captureNextAux_char_neg mem hn hnext hc] at hres
-    have inv' : UpperInv wf l r stack' := by
-      have reachable entry (mem : entry ∈ stack') : ∃ span, span.iterator = entry.it.it ∧ Path nfa wf l r span entry.state entry.update :=
+    have inv' : UpperInv wf it₀ stack' := by
+      have reachable entry (mem : entry ∈ stack') : Path nfa wf it₀ entry.it.it entry.state entry.update :=
         inv.reachable entry (by simp [mem])
       exact ⟨reachable⟩
     exact ih hres inv'
   | char_end visited update state it eq stack' mem visited' c state' hn hnext ih =>
     rw [captureNextAux_char_end mem hn hnext] at hres
-    have inv' : UpperInv wf l r stack' := by
-      have reachable entry (mem : entry ∈ stack') : ∃ span, span.iterator = entry.it.it ∧ Path nfa wf l r span entry.state entry.update :=
+    have inv' : UpperInv wf it₀ stack' := by
+      have reachable entry (mem : entry ∈ stack') : Path nfa wf it₀ entry.it.it entry.state entry.update :=
         inv.reachable entry (by simp [mem])
       exact ⟨reachable⟩
     exact ih hres inv'
   | sparse_pos visited update state it eq stack' mem visited' cs state' hn hnext hc ih =>
     rw [captureNextAux_sparse_pos mem hn hnext hc] at hres
-    have inv' : UpperInv wf l r (⟨update, state', it.next hnext, eq⟩ :: stack') := by
-      have reachable entry (mem : entry ∈ ⟨update, state', it.next hnext, eq⟩ :: stack') : ∃ span, span.iterator = entry.it.it ∧ Path nfa wf l r span entry.state entry.update := by
+    have inv' : UpperInv wf it₀ (⟨update, state', it.next hnext, eq⟩ :: stack') := by
+      have reachable entry (mem : entry ∈ ⟨update, state', it.next hnext, eq⟩ :: stack') : Path nfa wf it₀ entry.it.it entry.state entry.update := by
         simp at mem
         cases mem with
         | inl eq' =>
-          subst entry
-          have ⟨span, eqspan, path⟩ := inv.reachable ⟨update, state, it, eq⟩ (by simp)
-          simp at eqspan path
-          simp [BoundedIterator.hasNext, BoundedIterator.curr, ←eqspan] at hnext hc
-          have ⟨r', eqr'⟩ := span.exists_cons_of_curr' hnext rfl
-          refine ⟨span.next, by simp [span.next_iterator eqr', eqspan, BoundedIterator.next, String.Iterator.next'_eq_next], ?_⟩
-          simp
-          have step : NFA.Step nfa 0 state span state' span.next .none := by
-            simp [NFA.Step.iff_sparse hn, eqr', span.next_eq eqr', hc]
-          exact path.more step (by simp)
+          simp [eq']
+          have path := inv.reachable ⟨update, state, it, eq⟩ (by simp)
+          simp at path
+          have v : it.Valid := it.valid_of_it_valid path.validR
+          have ⟨l, r, vf⟩ := v.validFor_of_hasNext hnext
+          exact path.more (.sparse (Nat.zero_le _) state.isLt hn vf hc) (by simp)
         | inr mem => exact inv.reachable entry (by simp [mem])
       exact ⟨reachable⟩
     exact ih hres inv'
   | sparse_neg visited update state it eq stack' mem visited' cs state' hn hnext hc ih =>
     rw [captureNextAux_sparse_neg mem hn hnext hc] at hres
-    have inv' : UpperInv wf l r stack' := by
-      have reachable entry (mem : entry ∈ stack') : ∃ span, span.iterator = entry.it.it ∧ Path nfa wf l r span entry.state entry.update :=
+    have inv' : UpperInv wf it₀ stack' := by
+      have reachable entry (mem : entry ∈ stack') : Path nfa wf it₀ entry.it.it entry.state entry.update :=
         inv.reachable entry (by simp [mem])
       exact ⟨reachable⟩
     exact ih hres inv'
   | sparse_end visited update state it eq stack' mem visited' cs state' hn hnext ih =>
     rw [captureNextAux_sparse_end mem hn hnext] at hres
-    have inv' : UpperInv wf l r stack' := by
-      have reachable entry (mem : entry ∈ stack') : ∃ span, span.iterator = entry.it.it ∧ Path nfa wf l r span entry.state entry.update :=
+    have inv' : UpperInv wf it₀ stack' := by
+      have reachable entry (mem : entry ∈ stack') : Path nfa wf it₀ entry.it.it entry.state entry.update :=
         inv.reachable entry (by simp [mem])
       exact ⟨reachable⟩
     exact ih hres inv'
